examples/AutoSep.v
@@ -41,14 +41,14 @@ Require Import Bool.
 
 Ltac vcgen_simp := cbv beta iota zeta delta [map app imps
   LabelMap.add Entry Blocks Postcondition VerifCond
-  Straightline_ Seq_ Diverge_ Fail_ Skip_ Assert_ Use_
+  Straightline_ Seq_ Diverge_ Fail_ Skip_ Assert_
   Structured.If_ Structured.While_ Goto_ Structured.Call_ IGoto
   setArgs Programming.Reserved Programming.Formals Programming.Precondition
   importsMap fullImports buildLocals blocks union Nplus Nsucc length N_of_nat
   List.fold_left ascii_lt string_lt label'_lt
   LabelKey.compare' LabelKey.compare LabelKey.eq_dec
   LabelMap.find
-  toCmd Seq Instr Diverge Fail Skip Use_ Assert_
+  toCmd Seq Instr Diverge Fail Skip Assert_
   Programming.If_ Programming.While_ Goto Programming.Call_ RvImm'
   Assign' variableSlot' localsInvariant
   regInL lvalIn immInR labelIn variableSlot string_eq ascii_eq
@@ -68,6 +68,7 @@ Ltac vcgen_simp := cbv beta iota zeta delta [map app imps
   ZArith_dec.Zcompare_rec ZArith_dec.Z_ge_lt_dec BinInt.Z.compare ZArith_dec.Zcompare_rect
   ZArith_dec.Z_ge_dec label'_eq label'_rec label'_rect
   COperand1 CTest COperand2 Pos.succ
+  makeVcs
 ].
 
 Ltac vcgen :=
